Use named premises to make the proof more maintainable (#10)

Subtyping.v
@@ -34,12 +34,12 @@ Qed.
 
 (** Qualifier Ordering *)
 Inductive q_subtype : q -> q -> Prop :=
-  | q_refl : forall q1,
-      q1 <> Lost ->
+  | q_refl : forall q1
+      (Hnot_lost : q1 <> Lost),
       q_subtype q1 q1
   | q_rd : forall q1,
       q_subtype q1 RO
-  | q_bot: forall q1,
+  | q_bot : forall q1,
       q_subtype Bot q1
 where "q1 ⊑ q2" := (q_subtype q1 q2).
 Global Hint Constructors q_subtype: typ.
@@ -67,36 +67,35 @@ Definition parent_lookup (CT : class_table) (C : class_name) : option class_name
 
 (* Java base type subtyping *)
 Inductive base_subtype : class_table -> class_name -> class_name -> Prop :=
-  | base_refl : forall (CT : class_table) (C : class_name),
-      (* Reflexivity of base subtyping *)
-      C < dom CT ->
+  | base_refl : forall (CT : class_table) (C : class_name)
+      (Hdom : C < dom CT),
       base_subtype CT C C
-  | base_trans : forall (CT : class_table) (C D E : class_name),
-      base_subtype CT C D ->
-      base_subtype CT D E -> 
+  | base_trans : forall (CT : class_table) (C D E : class_name)
+      (Hsub1 : base_subtype CT C D)
+      (Hsub2 : base_subtype CT D E),
       base_subtype CT C E
-  | base_extends : forall (CT : class_table) (C D : class_name),
-      C < dom CT ->
-      D < dom CT ->
-      parent_lookup CT C = Some D ->
+  | base_extends : forall (CT : class_table) (C D : class_name)
+      (Hdom_C  : C < dom CT)
+      (Hdom_D  : D < dom CT)
+      (Hparent : parent_lookup CT C = Some D),
       base_subtype CT C D.
 Global Hint Constructors base_subtype: typ.
 
 (* Qualified type subtyping *)
 Inductive qualified_type_subtype : class_table -> qualified_type -> qualified_type -> Prop :=
-  | qtype_sub : forall CT qt1 qt2,
-	 		(sctype qt1) < (dom CT) ->
-      (sctype qt2) < (dom CT) ->
-      q_subtype (sqtype qt1) (sqtype qt2) ->
-      base_subtype CT (sctype qt1) (sctype qt2) ->
+  | qtype_sub : forall CT qt1 qt2
+      (Hdom1  : sctype qt1 < dom CT)
+      (Hdom2  : sctype qt2 < dom CT)
+      (Hqsub  : q_subtype (sqtype qt1) (sqtype qt2))
+      (Hbsub  : base_subtype CT (sctype qt1) (sctype qt2)),
       qualified_type_subtype CT qt1 qt2
-  | qtype_trans: forall CT qt1 qt2 qt3,
-      qualified_type_subtype CT qt1 qt2 ->
-      qualified_type_subtype CT qt2 qt3 ->
+  | qtype_trans : forall CT qt1 qt2 qt3
+      (Hsub12 : qualified_type_subtype CT qt1 qt2)
+      (Hsub23 : qualified_type_subtype CT qt2 qt3),
       qualified_type_subtype CT qt1 qt3
-  | qtype_refl: forall CT qt,
-      (sctype qt) < (dom CT) ->
-      sqtype qt <> Lost ->
+  | qtype_refl : forall CT qt
+      (Hdom      : sctype qt < dom CT)
+      (Hnot_lost : sqtype qt <> Lost),
       qualified_type_subtype CT qt qt.
 
 Lemma qualified_type_subtype_dom2 :
@@ -106,9 +105,9 @@ Lemma qualified_type_subtype_dom2 :
 Proof.
   intros CT qt1 qt2 H.
   induction H.
-  - assumption.
+  - exact Hdom2.
   - exact IHqualified_type_subtype2.
-  - assumption.
+  - exact Hdom.
 Qed.
 
 Lemma qualified_type_subtype_dom1 :
@@ -118,9 +117,9 @@ Lemma qualified_type_subtype_dom1 :
 Proof.
   intros CT qt1 qt2 H.
   induction H.
-  - assumption.
+  - exact Hdom1.
   - exact IHqualified_type_subtype1.
-  - assumption.
+  - exact Hdom.
 Qed.
 
 Lemma qualified_type_subtype_base_subtype :
@@ -128,13 +127,11 @@ Lemma qualified_type_subtype_base_subtype :
     qualified_type_subtype CT qt1 qt2 ->
     base_subtype CT (sctype qt1) (sctype qt2).
 Proof.
-    intros CT qt1 qt2 H.
-    induction H.
-    generalize dependent qt1.
-    generalize dependent qt2.
-    - intros. exact H2.
-    - eapply base_trans; eauto.
-    - eapply base_refl; eauto.
+  intros CT qt1 qt2 H.
+  induction H.
+  - exact Hbsub.
+  - eapply base_trans; eauto.
+  - eapply base_refl; eauto.
 Qed.
 
 Lemma qualified_type_subtype_q_subtype :
@@ -144,18 +141,11 @@ Lemma qualified_type_subtype_q_subtype :
 Proof.
   intros CT qt1 qt2 H.
   induction H.
-  - (* qtype_sub case *)
-    intros. exact H1.
-  - (* qtype_trans case *)
-  eapply q_subtype_trans; eauto.
-  - (* qtype_refl case *)
-    intros. 
-    destruct qt as [q c]; simpl.
+  - exact Hqsub.
+  - eapply q_subtype_trans; eauto.
+  - destruct qt as [q c]; simpl.
     destruct q; try (apply q_refl; discriminate).
-    exfalso.
-    simpl in H0.
-    apply H0.
-    reflexivity.
+    exfalso. simpl in Hnot_lost. apply Hnot_lost. reflexivity.
 Qed.
 
 Lemma base_subtype_domain : forall CT C D,
@@ -164,10 +154,8 @@ Lemma base_subtype_domain : forall CT C D,
 Proof.
   intros CT C D Hsub.
   induction Hsub.
-  - (* Reflexive *) 
-    split; exact H.
-  - (* Transitive *)
-    destruct IHHsub1 as [HC HD].
+  - split; exact Hdom.
+  - destruct IHHsub1 as [HC HD].
     destruct IHHsub2 as [_ HE].
     split; auto.
   - split; auto.
