Reachability.v
@@ -8,51 +8,41 @@ Import ListNotations.
 From RecordUpdate Require Import RecordUpdate.
 Require Import Syntax Typing Subtyping ViewpointAdaptation Helpers.
 
-Inductive reachable (h : heap): Loc -> Loc -> Prop :=
+Inductive reachable (h : heap) : Loc -> Loc -> Prop :=
 
-| rch_heap:
-    forall l,
-      l < dom h ->
+  | rch_heap : forall l
+      (Hdom : l < dom h),
       reachable h l l
 
-| rch_step:
-    forall l0 l1 obj f,
-      l1 < dom h ->
-      runtime_getObj h l0 = Some obj ->
-      getVal obj.(fields_map) f = Some (Iot l1) ->
+  | rch_step : forall l0 l1 obj f
+      (Hdom    : l1 < dom h)
+      (Hobj    : runtime_getObj h l0 = Some obj)
+      (Hfield  : getVal obj.(fields_map) f = Some (Iot l1)),
       reachable h l0 l1
 
-| rch_trans:
-    forall l0 l1 l2,
-      reachable h l0 l1 ->
-      reachable h l1 l2 ->
+  | rch_trans : forall l0 l1 l2
+      (Hreach1 : reachable h l0 l1)
+      (Hreach2 : reachable h l1 l2),
       reachable h l0 l2.
 
 
 Inductive reachable_abs (CT : class_table) (h : heap) : Loc -> Loc -> Prop :=
 
-| reachable_abs_heap :
-    forall l,
-      l < dom h ->
+  | reachable_abs_heap : forall l
+      (Hdom : l < dom h),
       reachable_abs CT h l l
 
-| reachable_abs_step :
-    forall l0 l1 any C vals k,
-      (* concrete step, as in [rch_step] *)
-      l1 < dom h ->
-      runtime_getObj h l0 = Some (mkObj (mkruntime_type any C) vals) ->
-      (* field [f] corresponds to index [k] and is RDM/Imm in the abstract state *)
-      nth_error vals k = Some (Iot l1) ->
-      (sf_mutability_rel CT C k RDM_f \/
-       sf_mutability_rel CT C k Imm_f) ->
-      (sf_assignability_rel CT C k RDA \/
-      sf_assignability_rel CT C k Final) ->
+  | reachable_abs_step : forall l0 l1 any C vals k
+      (Hdom        : l1 < dom h)
+      (Hobj        : runtime_getObj h l0 = Some (mkObj (mkruntime_type any C) vals))
+      (Hfield      : nth_error vals k = Some (Iot l1))
+      (Hmut_abs    : sf_mutability_rel CT C k RDM_f \/ sf_mutability_rel CT C k Imm_f)
+      (Hassign_abs : sf_assignability_rel CT C k RDA \/ sf_assignability_rel CT C k Final),
       reachable_abs CT h l0 l1
 
-| reachable_abs_trans :
-    forall l0 l1 l2,
-      reachable_abs CT h l0 l1 ->
-      reachable_abs CT h l1 l2 ->
+  | reachable_abs_trans : forall l0 l1 l2
+      (Hreach1 : reachable_abs CT h l0 l1)
+      (Hreach2 : reachable_abs CT h l1 l2),
       reachable_abs CT h l0 l2.
 
 Definition protected_locset
